Prefix: : <http://www.w3.org/2002/07/owl#>
Prefix: cc: <http://creativecommons.org/ns#>
Prefix: dc: <http://purl.org/dc/terms/>
Prefix: foaf: <http://xmlns.com/foaf/0.1/>
Prefix: geo: <http://www.w3.org/2003/01/geo/wgs84_pos/>
Prefix: om: <http://purl.oclc.org/net/unis/ontology/sensordata.owl/>
Prefix: owl: <http://www.w3.org/2002/07/owl#>
Prefix: rdf: <http://www.w3.org/1999/02/22-rdf-syntax-ns#>
Prefix: rdfs: <http://www.w3.org/2000/01/rdf-schema#>
Prefix: time: <http://www.w3.org/2006/time#>
Prefix: toco: <http://purl.org/toco/>
Prefix: units: <https://sweet.jpl.nasa.gov/>
Prefix: vann: <http://purl.org/vacob/vann/>
Prefix: xml: <http://www.w3.org/XML/1998/namespace>
Prefix: xsd: <http://www.w3.org/2001/XMLSchema#>



Ontology: <http://purl.org/toco/>


Annotations: 
    cc:license <http://creativecommons.org/licenses/by/3.0/>,
    dc:contributor <http://www.macs.hw.ac.uk/~ajg33/>,
    dc:contributor <https://www.eng.ed.ac.uk/about/people/mr-mohammad-dehghani-soltani>,
    dc:contributor <https://www.hw.ac.uk/staff/uk/eps/stephen-mclaughlin.htm>,
    dc:creator <https://www.gla.ac.uk/schools/computing/staff/qianruzhou/>,
    dc:description "A ontology developed for telecommunciation network systems with hybrid technologies, e.g., WiFi, LiFi, LTE, 2G/3G, optical, etc.",
    dc:issued "2015-3-1"^^xsd:date,
    dc:modified "2019-3-29"^^xsd:date,
    dc:publisher <http://hw.ac.uk>,
    dc:rights "Copyright  Â© 2015 Qianru Zhou",
    dc:title "Toucan Ontology"@en,
    vann:preferredNamespacePrefix "toco",
    vann:preferredNamespaceUri "http://purl.org/toco/",
    rdfs:comment "Version 1.1: creation"@en,
    owl:versionInfo 1.1

AnnotationProperty: cc:license

    
AnnotationProperty: dc:contributor

    
AnnotationProperty: dc:creator

    
AnnotationProperty: dc:description

    
AnnotationProperty: dc:issued

    
AnnotationProperty: dc:modified

    
AnnotationProperty: dc:publisher

    
AnnotationProperty: dc:rights

    
AnnotationProperty: dc:title

    
AnnotationProperty: owl:versionInfo

    
AnnotationProperty: rdfs:comment

    
AnnotationProperty: rdfs:isDefinedBy

    
AnnotationProperty: rdfs:label

    
AnnotationProperty: toco:contributor

    
AnnotationProperty: toco:license

    
AnnotationProperty: vann:preferredNamespacePrefix

    
AnnotationProperty: vann:preferredNamespaceUri

    
Datatype: rdf:PlainLiteral

    
Datatype: rdfs:Literal

    
Datatype: xsd:boolean

    
Datatype: xsd:dateTime

    
Datatype: xsd:float

    
Datatype: xsd:int

    
Datatype: xsd:string

    
ObjectProperty: <http://www.w3.org/2003/01/geo/wgs84_pos#location>

    Annotations: 
        rdfs:comment "The relation between something and the point, 
 or other geometrical thing in space, where it is.  For example, the realtionship between
 a radio tower and a Point with a given lat and long.
 Or a relationship between a park and its outline as a closed arc of points, or a road and
 its location as a arc (a sequence of points).
 Clearly in practice there will be limit to the accuracy of any such statement, but one would expect
 an accuracy appropriate for the size of the object and uses such as mapping .",
        rdfs:isDefinedBy <http://www.w3.org/2003/01/geo/wgs84_pos#>
    
    Domain: 
        toco:Device
    
    Range: 
        <http://www.w3.org/2003/01/geo/wgs84_pos#SpartialThing>
    
    
ObjectProperty: om:hasUnits

    Annotations: 
        rdfs:comment "the unit of an observation or measurement."^^xsd:string,
        rdfs:isDefinedBy <http://purl.org/toco/>
    
    Domain: 
        om:ObervationAndMeasurement
    
    Range: 
        <http://purl.obolibrary.org/obo/uo.owl/unit>
    
    
ObjectProperty: owl:topObjectProperty

    
ObjectProperty: toco:apsInRange

    Annotations: 
        rdfs:isDefinedBy <http://purl.org/toco/>
    
    Domain: 
        toco:UserDevice
    
    Range: 
        toco:AccessPoint
    
    
ObjectProperty: toco:belongsTo

    Annotations: 
        rdfs:isDefinedBy <http://purl.org/toco/>
    
    Domain: 
        toco:UserDevice
    
    Range: 
        toco:User
    
    InverseOf: 
        toco:hasDevice
    
    
ObjectProperty: toco:from

    Annotations: 
        rdfs:comment "the source node that the link is transmit from."^^xsd:string,
        rdfs:isDefinedBy <http://purl.org/toco/>
    
    SubPropertyOf: 
        owl:topObjectProperty
    
    Domain: 
        toco:Link
    
    Range: 
        toco:Interface
    
    
ObjectProperty: toco:hasAssociatedStations

    Annotations: 
        rdfs:comment "in wireless networks, the user equipments (mobile stations in another term, e.g., phones, laptops, tablets, etc.) that are associated to the access point."^^xsd:string,
        rdfs:isDefinedBy <http://purl.org/toco/>
    
    SubPropertyOf: 
        owl:topObjectProperty
    
    Domain: 
        toco:AccessPoint
    
    Range: 
        toco:UserDevice
    
    
ObjectProperty: toco:hasBandwidth

    Annotations: 
        rdfs:comment "the bandwidth of the link"^^xsd:string,
        rdfs:isDefinedBy <http://purl.org/toco/>
    
    SubPropertyOf: 
        toco:hasLinkProperty
    
    Domain: 
        toco:Link
    
    Range: 
        om:ObervationAndMeasurement
    
    
ObjectProperty: toco:hasDatarate

    Annotations: 
        rdfs:isDefinedBy <http://purl.org/toco/>
    
    SubPropertyOf: 
        toco:hasLinkProperty
    
    Domain: 
        toco:Link
    
    Range: 
        om:ObervationAndMeasurement
    
    
ObjectProperty: toco:hasDevice

    Annotations: 
        rdfs:isDefinedBy <http://purl.org/toco/>
    
    Domain: 
        toco:User
    
    Range: 
        toco:UserDevice
    
    InverseOf: 
        toco:belongsTo
    
    
ObjectProperty: toco:hasDistance

    Annotations: 
        rdfs:comment "the Euclidean distance between the LiFi user equipment and access point."^^xsd:string,
        rdfs:isDefinedBy <http://purl.org/toco/>
    
    SubPropertyOf: 
        toco:hasLiFiAssociationProperty
    
    Domain: 
        toco:LiFiAssociation
    
    
ObjectProperty: toco:hasFlow

    Annotations: 
        rdfs:isDefinedBy <http://purl.org/toco/>
    
    Domain: 
        toco:SystemDevice
    
    Range: 
        toco:Flow
    
    
ObjectProperty: toco:hasFlowAction

    Annotations: 
        rdfs:isDefinedBy <http://purl.org/toco/>
    
    Domain: 
        toco:Flow
    
    Range: 
        toco:Action
    
    
ObjectProperty: toco:hasIncidentAngle

    Annotations: 
        rdfs:comment "The angle of incidence of the LED receiver on LiFi user equipment, which is the angle between the visiable light ray incident on a surface and the line perpendicular to the surface at the point of incidence, called the normal."^^xsd:string,
        rdfs:isDefinedBy <http://purl.org/toco/>
    
    SubPropertyOf: 
        toco:hasLiFiAssociationProperty
    
    Domain: 
        toco:LiFiAssociation
    
    
ObjectProperty: toco:hasInterface

    Annotations: 
        rdfs:comment "the fact that a device has a interface."^^xsd:string,
        rdfs:isDefinedBy <http://purl.org/toco/>
    
    Domain: 
        toco:Device
    
    Range: 
        toco:Interface
    
    InverseOf: 
        toco:isIn
    
    
ObjectProperty: toco:hasLTEAssociation

    SubPropertyOf: 
        toco:hasWirelessAssociation
    
    Range: 
        toco:LTEAssociation
    
    
ObjectProperty: toco:hasLiFiAssociation

    SubPropertyOf: 
        toco:hasWirelessAssociation
    
    Domain: 
        toco:LiFiWLAN
    
    Range: 
        toco:LiFiAssociation
    
    
ObjectProperty: toco:hasLiFiAssociationProperty

    Annotations: 
        rdfs:comment "The properties of the visiable light association between the LED on LiFi access point and LiFi user equipment."^^xsd:string
    
    SubPropertyOf: 
        toco:hasWirelessLinkProperty
    
    Domain: 
        toco:LiFiAssociation
    
    
ObjectProperty: toco:hasLiFiWLAN

    SubPropertyOf: 
        toco:hasWLAN
    
    Domain: 
        toco:Device
    
    Range: 
        toco:LiFiWLAN
    
    
ObjectProperty: toco:hasLink

    Annotations: 
        rdfs:isDefinedBy <http://purl.org/toco/>
    
    Domain: 
        toco:Interface
    
    Range: 
        toco:Link
    
    
ObjectProperty: toco:hasLinkProperty

    Annotations: 
        rdfs:isDefinedBy <http://purl.org/toco/>
    
    Domain: 
        toco:Link
    
    
ObjectProperty: toco:hasPort

    SubPropertyOf: 
        toco:hasInterface
    
    Domain: 
        toco:Device
    
    Range: 
        toco:Interface
    
    
ObjectProperty: toco:hasRadianceAngle

    Annotations: 
        rdfs:comment "the radiance angle of the light ray transmitted from LED on LiFi access point."^^xsd:string,
        rdfs:isDefinedBy <http://purl.org/toco/>
    
    SubPropertyOf: 
        toco:hasLiFiAssociationProperty
    
    Domain: 
        toco:LiFiAssociation
    
    
ObjectProperty: toco:hasRoundTripTime

    Annotations: 
        rdfs:comment "the round trip time of a link, which is the time taken for signal travel a round trip via this link."^^xsd:string
    
    SubPropertyOf: 
        toco:hasLinkProperty
    
    Domain: 
        toco:Link
    
    Range: 
        om:ObervationAndMeasurement
    
    
ObjectProperty: toco:hasSatelliteAssociation

    SubPropertyOf: 
        toco:hasWirelessAssociation
    
    Domain: 
        toco:Device
    
    Range: 
        toco:SatelliteAssociation
    
    
ObjectProperty: toco:hasService

    Annotations: 
        rdfs:isDefinedBy <http://purl.org/toco/>
    
    Domain: 
        toco:UserDevice
    
    Range: 
        toco:Service
    
    
ObjectProperty: toco:hasStandardDeviation

    Annotations: 
        rdfs:comment "After multiple round trip time tested on a link, the deviation of these test results."^^xsd:string
    
    SubPropertyOf: 
        toco:hasLinkProperty
    
    Domain: 
        toco:Link
    
    Range: 
        om:ObervationAndMeasurement
    
    
ObjectProperty: toco:hasThroughPut

    SubPropertyOf: 
        toco:hasLinkProperty
    
    Domain: 
        toco:Link
    
    Range: 
        om:ObervationAndMeasurement
    
    
ObjectProperty: toco:hasTransmitPower

    Annotations: 
        rdfs:isDefinedBy <http://purl.org/toco/>
    
    SubPropertyOf: 
        owl:topObjectProperty
    
    Domain: 
        toco:Interface
    
    Range: 
        om:ObervationAndMeasurement
    
    
ObjectProperty: toco:hasTxpower

    Annotations: 
        rdfs:isDefinedBy <http://purl.org/toco/>
    
    SubPropertyOf: 
        toco:hasLinkProperty
    
    Domain: 
        toco:Link
    
    Range: 
        om:ObervationAndMeasurement
    
    
ObjectProperty: toco:hasUserDeviceStatus

    Domain: 
        toco:UserDevice
    
    Range: 
        toco:UserDeviceStatus
    
    
ObjectProperty: toco:hasWLAN

    SubPropertyOf: 
        toco:hasInterface
    
    Domain: 
        toco:Device
    
    Range: 
        toco:WLAN
    
    
ObjectProperty: toco:hasWiFiAssociation

    SubPropertyOf: 
        toco:hasWirelessAssociation
    
    Domain: 
        toco:WiFiWLAN
    
    Range: 
        toco:WiFiAssociation
    
    
ObjectProperty: toco:hasWiFiWLAN

    SubPropertyOf: 
        toco:hasWLAN
    
    Domain: 
        toco:Device
    
    Range: 
        toco:WiFiWLAN
    
    
ObjectProperty: toco:hasWiredLink

    SubPropertyOf: 
        toco:hasLink
    
    DisjointWith: 
        toco:hasWirelessAssociation
    
    Domain: 
        toco:Interface
    
    Range: 
        toco:WiredLink
    
    
ObjectProperty: toco:hasWirelessAssociation

    SubPropertyOf: 
        toco:hasLink
    
    DisjointWith: 
        toco:hasWiredLink
    
    Domain: 
        toco:WLAN
    
    Range: 
        toco:WirelessAssociation
    
    
ObjectProperty: toco:hasWirelessLinkProperty

    SubPropertyOf: 
        toco:hasLinkProperty
    
    Domain: 
        toco:WirelessAssociation
    
    
ObjectProperty: toco:isIn

    Annotations: 
        rdfs:comment "the relation that a interface belongs to a device. A device can have multiple interfaces, but a interface can be in one and only one device."^^xsd:string,
        rdfs:isDefinedBy <http://purl.org/toco/>
    
    Domain: 
        toco:Interface
    
    Range: 
        toco:Device
    
    InverseOf: 
        toco:hasInterface
    
    
ObjectProperty: toco:range

    Annotations: 
        rdfs:comment "the signal range of wireless devices, such as WiFi access point, LiFi access point, WiFi mobile station, and LiFi mobile station."^^xsd:string,
        rdfs:isDefinedBy <http://purl.org/toco/>
    
    Domain: 
        toco:Device
    
    Range: 
        om:ObervationAndMeasurement
    
    
ObjectProperty: toco:stationsInRange

    Annotations: 
        rdfs:comment "in wireless networks (WiFi/LiFi), the mobile stations in the range of the access points."^^xsd:string,
        rdfs:isDefinedBy <http://purl.org/toco/>
    
    Domain: 
        toco:AccessPoint
    
    Range: 
        toco:UserEquipment
    
    
ObjectProperty: toco:to

    Annotations: 
        rdfs:comment "the destination node of the link."^^xsd:string,
        rdfs:isDefinedBy <http://purl.org/toco/>
    
    SubPropertyOf: 
        owl:topObjectProperty
    
    Domain: 
        toco:Link
    
    Range: 
        toco:Interface
    
    
DataProperty: <http://www.w3.org/2003/01/geo/wgs84_pos#alt>

    Annotations: 
        rdfs:comment "the altitude of a spartial thing, i.e., a point.",
        rdfs:isDefinedBy <http://www.w3.org/2003/01/geo/wgs84_pos#>
    
    Domain: 
        <http://www.w3.org/2003/01/geo/wgs84_pos#SpartialThing>
    
    Range: 
        xsd:float
    
    
DataProperty: <http://www.w3.org/2003/01/geo/wgs84_pos#lat>

    Annotations: 
        rdfs:isDefinedBy <http://www.w3.org/2003/01/geo/wgs84_pos#>,
        rdfs:isDefinedBy "the latitude of a point"
    
    Domain: 
        <http://www.w3.org/2003/01/geo/wgs84_pos#SpartialThing>
    
    Range: 
        xsd:float
    
    
DataProperty: <http://www.w3.org/2003/01/geo/wgs84_pos#long>

    Annotations: 
        rdfs:isDefinedBy <http://www.w3.org/2003/01/geo/wgs84_pos#>,
        rdfs:isDefinedBy "the longitude of a spartial thing, i.e., a point."
    
    Domain: 
        <http://www.w3.org/2003/01/geo/wgs84_pos#SpartialThing>
    
    Range: 
        xsd:float
    
    
DataProperty: foaf:firstName

    Annotations: 
        rdfs:comment "the first name of a user.",
        rdfs:isDefinedBy <http://xmlns.com/foaf/0.1/>
    
    Domain: 
        foaf:Person
    
    Range: 
        rdfs:Literal
    
    
DataProperty: foaf:gender

    Annotations: 
        rdfs:comment "the gender of a user, reused from foaf",
        rdfs:isDefinedBy <http://xmlns.com/foaf/0.1/>
    
    Domain: 
        foaf:Person
    
    Range: 
        rdfs:Literal
    
    
DataProperty: foaf:lastName

    Annotations: 
        rdfs:comment "the last name of a person.
Reused from foaf",
        rdfs:isDefinedBy <http://xmlns.com/foaf/0.1/>
    
    Domain: 
        foaf:Person
    
    Range: 
        rdfs:Literal
    
    
DataProperty: om:hasUnit

    Annotations: 
        rdfs:comment "reused from SENSEI Observation and Measurement Ontology."^^xsd:string,
        rdfs:isDefinedBy <http://purl.oclc.org/net/unis/ontology/sensordata.owl/>
    
    Domain: 
        om:ObervationAndMeasurement
    
    Range: 
        xsd:string
    
    
DataProperty: om:hasValue

    Annotations: 
        rdfs:comment "the value of an observation or measurement."^^xsd:string,
        rdfs:isDefinedBy <http://purl.org/toco/>
    
    Domain: 
        om:ObervationAndMeasurement
    
    Range: 
        xsd:float
    
    
DataProperty: toco:channel

    Annotations: 
        rdfs:comment "the channel id of a interface."^^xsd:string,
        rdfs:isDefinedBy <http://purl.org/toco/>
    
    Domain: 
        toco:Interface
    
    Range: 
        xsd:int
    
    
DataProperty: toco:cookie

    Annotations: 
        rdfs:isDefinedBy <http://purl.org/toco/>
    
    Domain: 
        toco:Flow
    
    Range: 
        xsd:string
    
    SubPropertyOf: 
        toco:hasFlowProperty
    
    
DataProperty: toco:dlDst

    Annotations: 
        rdfs:comment "the Ethernet destination address of the flow. It should be an MAC address, with 6 pairs of hexadecimal digits."
    
    Domain: 
        toco:Flow
    
    Range: 
        xsd:string
    
    SubPropertyOf: 
        toco:hasFlowProperty
    
    
DataProperty: toco:dlSrc

    Annotations: 
        rdfs:comment "the Ethernet source address of the flow. It should be an MAC address with 6 pairs of hexadecimal digits"
    
    Domain: 
        toco:Flow
    
    Range: 
        xsd:string
    
    SubPropertyOf: 
        toco:hasFlowProperty
    
    
DataProperty: toco:driver

    Domain: 
        toco:AccessPoint
    
    Range: 
        xsd:string
    
    
DataProperty: toco:flags

    Annotations: 
        rdfs:isDefinedBy <http://purl.org/toco/>
    
    Domain: 
        toco:Flow
    
    Range: 
        xsd:int
    
    SubPropertyOf: 
        toco:hasFlowProperty
    
    
DataProperty: toco:frequency

    Annotations: 
        rdfs:comment "the frequency of the radio wave transmitted by a wireless interface (WLAN)."^^xsd:string
    
    Domain: 
        toco:Interface
    
    Range: 
        xsd:float
    
    
DataProperty: toco:hardTimeout

    Annotations: 
        rdfs:isDefinedBy <http://purl.org/toco/>
    
    Domain: 
        toco:Flow
    
    Range: 
        xsd:string
    
    SubPropertyOf: 
        toco:hasFlowProperty
    
    
DataProperty: toco:hasAntennaGain

    Annotations: 
        rdfs:comment "the gain of an antenna on the wireless interface."^^xsd:string,
        rdfs:isDefinedBy <http://purl.org/toco/>
    
    Domain: 
        toco:WLAN
    
    Range: 
        xsd:int
    
    
DataProperty: toco:hasAntennaHeight

    Annotations: 
        rdfs:comment "the height of the antenna of a wireless interface"^^xsd:string,
        rdfs:isDefinedBy <http://purl.org/toco/>
    
    Domain: 
        toco:WLAN
    
    Range: 
        xsd:float
    
    
DataProperty: toco:hasDistance

    Annotations: 
        rdfs:comment "the Euclidean distance between the LiFi user equipment and access point."^^xsd:string,
        rdfs:isDefinedBy <http://purl.org/toco/>
    
    Range: 
        xsd:float
    
    
DataProperty: toco:hasErrorCode

    Annotations: 
        rdfs:comment "the error code of a service."^^xsd:string,
        rdfs:isDefinedBy <http://purl.org/toco/>
    
    Domain: 
        toco:Service
    
    Range: 
        xsd:string
    
    
DataProperty: toco:hasFieldOfView

    Annotations: 
        rdfs:comment "Field of view (FOV) is the open observable area where a LiFi user equipment could receive visiable light signal. It is defined by let the incident angle of the LiFi user equipment equals to Pi/2.

If the incident angle larger than Pi/2, the light ray is out of the FOV, thus cannot be received by the LiFi user equipment."^^xsd:string,
        rdfs:isDefinedBy <http://purl.org/toco/>
    
    Domain: 
        toco:LiFiUserEquipment
    
    Range: 
        xsd:float
    
    SubPropertyOf: 
        toco:hasLiFiUserEquipmentProperty
    
    
DataProperty: toco:hasFlowProperty

    Annotations: 
        rdfs:isDefinedBy <http://purl.org/toco/>
    
    
DataProperty: toco:hasGainOfConcentrator

    Annotations: 
        rdfs:comment "The gain of the concentrator on the LiFi user equipment, usually equals to 1."^^xsd:string,
        rdfs:isDefinedBy <http://purl.org/toco/>
    
    Domain: 
        toco:LiFiUserEquipment
    
    Range: 
        xsd:float
    
    SubPropertyOf: 
        toco:hasLiFiUserEquipmentProperty
    
    
DataProperty: toco:hasGainofOpticalFilter

    Annotations: 
        rdfs:comment "Gain of optical filter on LiFi access point."^^xsd:string,
        rdfs:isDefinedBy <http://purl.org/toco/>
    
    Domain: 
        toco:LiFiAccessPoint
    
    Range: 
        xsd:float
    
    SubPropertyOf: 
        toco:hasLiFiAccessPointProperty
    
    
DataProperty: toco:hasHalfIntensityAngle

    Annotations: 
        rdfs:comment "The angle of half intensity of the LED light transmiting visible light signal in a LiFi access point. 

A fixed value. It is the angle where the radiated intensity will be half as intense as it would be at 0 degrees, or pointing straight ahead.

Factors that contribute to the angle of half intensity include the amount of diffusing material in the epoxy, the shape of the reflector cup which surrounds the LED chip, the shape of the LED lens, the distance from the LED to the tip of the lens, and the type of emitter chip.

The most common value is Pi/3."^^xsd:string,
        rdfs:isDefinedBy <http://purl.org/toco/>
    
    Domain: 
        toco:LiFiAccessPoint
    
    Range: 
        xsd:float
    
    SubPropertyOf: 
        toco:hasLiFiAccessPointProperty
    
    
DataProperty: toco:hasIP

    Annotations: 
        rdfs:comment "the IP address of the interface."^^xsd:string,
        rdfs:isDefinedBy <http://purl.org/toco/>
    
    Domain: 
        toco:Interface
    
    Range: 
        xsd:string
    
    
DataProperty: toco:hasIncidentAngle

    Annotations: 
        rdfs:comment "The angle of incidence of the LED receiver on LiFi user equipment, which is the angle between the visiable light ray incident on a surface and the line perpendicular to the surface at the point of incidence, called the normal."^^xsd:string,
        rdfs:isDefinedBy <http://purl.org/toco/>
    
    Range: 
        xsd:float
    
    
DataProperty: toco:hasInterfaceName

    Annotations: 
        rdfs:comment "the port number of an interface"^^xsd:string,
        rdfs:isDefinedBy <http://purl.org/toco/>
    
    Domain: 
        toco:Interface
    
    Range: 
        xsd:string
    
    
DataProperty: toco:hasJoinDate

    Annotations: 
        rdfs:comment "the join date of the user device",
        rdfs:isDefinedBy <http://purl.org/toco/>
    
    Domain: 
        toco:UserDevice
    
    Range: 
        xsd:dateTime
    
    
DataProperty: toco:hasLiFiAccessPointProperty

    Annotations: 
        rdfs:comment "datatype properties dedicated for LiFi access points"^^xsd:string,
        rdfs:isDefinedBy <http://purl.org/toco/>
    
    Domain: 
        toco:LiFiAccessPoint
    
    Range: 
        xsd:float
    
    
DataProperty: toco:hasLiFiAssociationProperty

    Annotations: 
        rdfs:comment "The properties of the visiable light association between the LED on LiFi access point and LiFi user equipment."^^xsd:string
    
    Range: 
        xsd:float
    
    
DataProperty: toco:hasLiFiUserEquipmentProperty

    Annotations: 
        rdfs:comment "properties of LiFi user equipments."^^xsd:string,
        rdfs:isDefinedBy <http://purl.org/toco/>
    
    Domain: 
        toco:LiFiUserEquipment
    
    Range: 
        xsd:float
    
    
DataProperty: toco:hasLinkProperty

    Annotations: 
        rdfs:isDefinedBy <http://purl.org/toco/>
    
    Range: 
        xsd:float
    
    
DataProperty: toco:hasMAC

    Annotations: 
        rdfs:comment "the MAC address of the interface."^^xsd:string,
        rdfs:isDefinedBy <http://purl.org/toco/>
    
    Domain: 
        toco:Interface
    
    Range: 
        xsd:string
    
    
DataProperty: toco:hasOpticalTransmittedPower

    Annotations: 
        rdfs:comment "the transmitted power of the LED on the LiFi access point"^^xsd:string,
        rdfs:isDefinedBy <http://purl.org/toco/>
    
    Domain: 
        toco:LiFiAccessPoint
    
    Range: 
        xsd:float
    
    SubPropertyOf: 
        toco:hasLiFiAccessPointProperty
    
    
DataProperty: toco:hasPacketLoss

    Annotations: 
        rdfs:comment "the packet loss rate of a link, usually in percentage."^^xsd:string,
        rdfs:isDefinedBy <http://purl.org/toco/>
    
    Domain: 
        toco:Link
    
    Range: 
        xsd:float
    
    
DataProperty: toco:hasRadianceAngle

    Annotations: 
        rdfs:comment "the radiance angle of the light ray transmitted from LED on LiFi access point."^^xsd:string,
        rdfs:isDefinedBy <http://purl.org/toco/>
    
    Range: 
        xsd:float
    
    
DataProperty: toco:hasRespansivity

    Annotations: 
        rdfs:isDefinedBy <http://purl.org/toco/>
    
    Domain: 
        toco:LiFiAccessPoint
    
    Range: 
        xsd:float
    
    SubPropertyOf: 
        toco:hasLiFiAccessPointProperty
    
    
DataProperty: toco:hasServiceEndTime

    Annotations: 
        rdfs:comment "the time that a service ends."^^xsd:string,
        rdfs:isDefinedBy <http://purl.org/toco/>
    
    Domain: 
        toco:Service
    
    Range: 
        xsd:dateTime
    
    
DataProperty: toco:hasServiceStartTime

    Annotations: 
        rdfs:comment "the start time of a service."^^xsd:string,
        rdfs:isDefinedBy <http://purl.org/toco/>
    
    Domain: 
        toco:Service
    
    Range: 
        xsd:dateTime
    
    
DataProperty: toco:hasServiceStatus

    Annotations: 
        rdfs:comment "the status of the service."^^xsd:string,
        rdfs:isDefinedBy <http://purl.org/toco/>
    
    Domain: 
        toco:Service
    
    Range: 
        xsd:string
    
    
DataProperty: toco:hasServiceType

    Annotations: 
        rdfs:comment "the type of communication services, e.g., video, audio, file transmit, text transmiting, etc."^^xsd:string,
        rdfs:isDefinedBy <http://purl.org/toco/>
    
    Domain: 
        toco:Service
    
    Range: 
        xsd:string
    
    
DataProperty: toco:hasUserID

    Annotations: 
        rdfs:comment "the user ID of the user",
        rdfs:isDefinedBy <http://purl.org/toco/>
    
    Domain: 
        toco:User
    
    Range: 
        xsd:string
    
    
DataProperty: toco:hasWirelessLinkProperty

    Range: 
        xsd:float
    
    
DataProperty: toco:idleTimeout

    Annotations: 
        rdfs:isDefinedBy <http://purl.org/toco/>
    
    Domain: 
        toco:Flow
    
    Range: 
        xsd:string
    
    SubPropertyOf: 
        toco:hasFlowProperty
    
    
DataProperty: toco:inPort

    Annotations: 
        rdfs:comment "the port number of the in port of the flow, or could be a keyword, such as \"LOCAL\""
    
    Domain: 
        toco:Flow
    
    Range: 
        xsd:string
    
    SubPropertyOf: 
        toco:hasFlowProperty
    
    
DataProperty: toco:isUP

    Annotations: 
        rdfs:comment "indicate whether a interface is up or not.",
        rdfs:isDefinedBy <http://purl.org/toco/>
    
    Domain: 
        toco:Interface
    
    Range: 
        xsd:boolean
    
    
DataProperty: toco:mode

    Domain: 
        toco:Interface
    
    Range: 
        xsd:int
    
    
DataProperty: toco:nwProtocol

    Annotations: 
        rdfs:comment "network protocol. The nw_proto property of a flow."
    
    Domain: 
        toco:Flow
    
    Range: 
        xsd:string
    
    SubPropertyOf: 
        toco:hasFlowProperty
    
    
DataProperty: toco:nwTos

    Annotations: 
        rdfs:comment "network type of service. the nw_tos property of a flow. It should be a decimal number with the value between 0-255."
    
    Domain: 
        toco:Flow
    
    Range: 
        xsd:int
    
    SubPropertyOf: 
        toco:hasFlowProperty
    
    
DataProperty: toco:priority

    Annotations: 
        rdfs:isDefinedBy <http://purl.org/toco/>
    
    Domain: 
        toco:Flow
    
    Range: 
        xsd:string
    
    SubPropertyOf: 
        toco:hasFlowProperty
    
    
DataProperty: toco:ssid

    Annotations: 
        rdfs:comment "in wireless networks, the ssid of the network this device belongs to."^^xsd:string,
        rdfs:isDefinedBy <http://purl.org/toco/>
    
    Domain: 
        toco:Device
    
    Range: 
        xsd:string
    
    
DataProperty: toco:tableId

    Annotations: 
        rdfs:isDefinedBy <http://purl.org/toco/>
    
    Domain: 
        toco:Flow
    
    Range: 
        xsd:string
    
    SubPropertyOf: 
        toco:hasFlowProperty
    
    
DataProperty: toco:toPort

    Annotations: 
        rdfs:comment "the port number of the port forward to defined by the to_port property of the flow action OUTPUT."
    
    Domain: 
        toco:Action
    
    Range: 
        xsd:string
    
    
Class: <http://purl.obolibrary.org/obo/UO_0000001>

    Annotations: 
        rdfs:isDefinedBy <http://purl.obolibrary.org/obo/uo.owl>,
        rdfs:label "length unit"
    
    SubClassOf: 
        <http://purl.obolibrary.org/obo/uo.owl/unit>
    
    
Class: <http://purl.obolibrary.org/obo/UO_0000003>

    Annotations: 
        rdfs:isDefinedBy <http://purl.obolibrary.org/obo/uo.owl>,
        rdfs:label "time unit"
    
    SubClassOf: 
        <http://purl.obolibrary.org/obo/uo.owl/unit>
    
    
Class: <http://purl.obolibrary.org/obo/UO_0000008>

    Annotations: 
        rdfs:isDefinedBy <http://purl.obolibrary.org/obo/uo.owl>,
        rdfs:label "meter"
    
    SubClassOf: 
        <http://purl.obolibrary.org/obo/UO_0000001>
    
    
Class: <http://purl.obolibrary.org/obo/UO_0000010>

    Annotations: 
        rdfs:isDefinedBy <http://purl.obolibrary.org/obo/uo.owl>,
        rdfs:label "second"
    
    SubClassOf: 
        <http://purl.obolibrary.org/obo/UO_0000003>
    
    
Class: <http://purl.obolibrary.org/obo/UO_0000016>

    Annotations: 
        rdfs:isDefinedBy <http://purl.obolibrary.org/obo/uo.owl>,
        rdfs:label "millimeter"
    
    SubClassOf: 
        <http://purl.obolibrary.org/obo/UO_0000001>
    
    
Class: <http://purl.obolibrary.org/obo/UO_0000017>

    Annotations: 
        rdfs:isDefinedBy <http://purl.obolibrary.org/obo/uo.owl>,
        rdfs:label "micrometer"
    
    SubClassOf: 
        <http://purl.obolibrary.org/obo/UO_0000001>
    
    
Class: <http://purl.obolibrary.org/obo/UO_0000028>

    Annotations: 
        rdfs:isDefinedBy <http://purl.obolibrary.org/obo/uo.owl>,
        rdfs:label "millisecond"
    
    SubClassOf: 
        <http://purl.obolibrary.org/obo/UO_0000003>
    
    
Class: <http://purl.obolibrary.org/obo/UO_0000031>

    Annotations: 
        rdfs:isDefinedBy <http://purl.obolibrary.org/obo/uo.owl>,
        rdfs:label "minute"
    
    SubClassOf: 
        <http://purl.obolibrary.org/obo/UO_0000003>
    
    
Class: <http://purl.obolibrary.org/obo/UO_0000032>

    Annotations: 
        rdfs:isDefinedBy <http://purl.obolibrary.org/obo/uo.owl>,
        rdfs:label "hour"
    
    SubClassOf: 
        <http://purl.obolibrary.org/obo/UO_0000003>
    
    
Class: <http://purl.obolibrary.org/obo/UO_0000034>

    Annotations: 
        rdfs:isDefinedBy <http://purl.obolibrary.org/obo/uo.owl>,
        rdfs:label "week"
    
    SubClassOf: 
        <http://purl.obolibrary.org/obo/UO_0000003>
    
    
Class: <http://purl.obolibrary.org/obo/UO_0000035>

    Annotations: 
        rdfs:isDefinedBy <http://purl.obolibrary.org/obo/uo.owl>,
        rdfs:label "month"
    
    SubClassOf: 
        <http://purl.obolibrary.org/obo/UO_0000003>
    
    
Class: <http://purl.obolibrary.org/obo/UO_0000036>

    Annotations: 
        rdfs:isDefinedBy <http://purl.obolibrary.org/obo/uo.owl>,
        rdfs:label "year"
    
    SubClassOf: 
        <http://purl.obolibrary.org/obo/UO_0000003>
    
    
Class: <http://purl.obolibrary.org/obo/UO_0000058>

    Annotations: 
        rdfs:isDefinedBy <http://purl.obolibrary.org/obo/uo.owl>,
        rdfs:label "rotational frequency unit"
    
    SubClassOf: 
        <http://purl.obolibrary.org/obo/UO_0000105>
    
    
Class: <http://purl.obolibrary.org/obo/UO_0000060>

    Annotations: 
        rdfs:isDefinedBy <http://purl.obolibrary.org/obo/uo.owl>,
        rdfs:label "speed/velocity unit"
    
    SubClassOf: 
        <http://purl.obolibrary.org/obo/uo.owl/unit>
    
    
Class: <http://purl.obolibrary.org/obo/UO_0000092>

    Annotations: 
        rdfs:isDefinedBy <http://purl.obolibrary.org/obo/uo.owl>,
        rdfs:label "turns per second"
    
    SubClassOf: 
        <http://purl.obolibrary.org/obo/UO_0000058>
    
    
Class: <http://purl.obolibrary.org/obo/UO_0000094>

    Annotations: 
        rdfs:isDefinedBy <http://purl.obolibrary.org/obo/uo.owl>,
        rdfs:label "meter per second"
    
    SubClassOf: 
        <http://purl.obolibrary.org/obo/UO_0000060>
    
    
Class: <http://purl.obolibrary.org/obo/UO_0000105>

    Annotations: 
        rdfs:label "frequency unit"
    
    SubClassOf: 
        <http://purl.obolibrary.org/obo/uo.owl/unit>
    
    
Class: <http://purl.obolibrary.org/obo/UO_0000106>

    Annotations: 
        rdfs:isDefinedBy <http://purl.obolibrary.org/obo/uo.owl>,
        rdfs:label "hertz"
    
    SubClassOf: 
        <http://purl.obolibrary.org/obo/UO_0000105>
    
    
Class: <http://purl.obolibrary.org/obo/UO_0000111>

    Annotations: 
        rdfs:isDefinedBy <http://purl.obolibrary.org/obo/uo.owl>,
        rdfs:label "energy unit"
    
    SubClassOf: 
        <http://purl.obolibrary.org/obo/uo.owl/unit>
    
    
Class: <http://purl.obolibrary.org/obo/UO_0000113>

    Annotations: 
        rdfs:label "power unit"
    
    SubClassOf: 
        <http://purl.obolibrary.org/obo/uo.owl/unit>
    
    
Class: <http://purl.obolibrary.org/obo/UO_0000114>

    Annotations: 
        rdfs:isDefinedBy <http://purl.obolibrary.org/obo/uo.owl>,
        rdfs:label "watt"
    
    SubClassOf: 
        <http://purl.obolibrary.org/obo/UO_0000113>
    
    
Class: <http://purl.obolibrary.org/obo/UO_0000223>

    Annotations: 
        rdfs:isDefinedBy <http://purl.obolibrary.org/obo/uo.owl>,
        rdfs:label "watt-hour"
    
    SubClassOf: 
        <http://purl.obolibrary.org/obo/UO_0000111>
    
    
Class: <http://purl.obolibrary.org/obo/UO_0000224>

    Annotations: 
        rdfs:isDefinedBy <http://purl.obolibrary.org/obo/uo.owl>,
        rdfs:label "kilowatt-hour"
    
    SubClassOf: 
        <http://purl.obolibrary.org/obo/UO_0000111>
    
    
Class: <http://purl.obolibrary.org/obo/UO_0000231>

    Annotations: 
        rdfs:isDefinedBy <http://purl.obolibrary.org/obo/uo.owl>,
        rdfs:label "information unit"
    
    SubClassOf: 
        <http://purl.obolibrary.org/obo/uo.owl/unit>
    
    
Class: <http://purl.obolibrary.org/obo/UO_0000232>

    Annotations: 
        rdfs:isDefinedBy <http://purl.obolibrary.org/obo/uo.owl>,
        rdfs:label "bit"
    
    SubClassOf: 
        <http://purl.obolibrary.org/obo/UO_0000231>
    
    
Class: <http://purl.obolibrary.org/obo/UO_0000233>

    Annotations: 
        rdfs:isDefinedBy <http://purl.obolibrary.org/obo/uo.owl>,
        rdfs:label "byte"
    
    SubClassOf: 
        <http://purl.obolibrary.org/obo/UO_0000231>
    
    
Class: <http://purl.obolibrary.org/obo/UO_0000235>

    Annotations: 
        rdfs:isDefinedBy <http://purl.obolibrary.org/obo/uo.owl>,
        rdfs:label "megabyte"
    
    SubClassOf: 
        <http://purl.obolibrary.org/obo/UO_0000231>
    
    
Class: <http://purl.obolibrary.org/obo/UO_0000325>

    Annotations: 
        rdfs:isDefinedBy <http://purl.obolibrary.org/obo/uo.owl>,
        rdfs:label "megaHertz"
    
    SubClassOf: 
        <http://purl.obolibrary.org/obo/UO_0000105>
    
    
Class: <http://purl.obolibrary.org/obo/UO_0000331>

    Annotations: 
        rdfs:isDefinedBy <http://purl.obolibrary.org/obo/uo.owl>,
        rdfs:label "gigabyte"
    
    SubClassOf: 
        <http://purl.obolibrary.org/obo/UO_0000231>
    
    
Class: <http://purl.obolibrary.org/obo/UO_0000332>

    Annotations: 
        rdfs:isDefinedBy <http://purl.obolibrary.org/obo/uo.owl>,
        rdfs:label "terabyte"
    
    SubClassOf: 
        <http://purl.obolibrary.org/obo/UO_0000231>
    
    
Class: <http://purl.obolibrary.org/obo/UO_0010005>

    Annotations: 
        rdfs:isDefinedBy <http://purl.obolibrary.org/obo/uo.owl>,
        rdfs:label "millimeters per day"
    
    SubClassOf: 
        <http://purl.obolibrary.org/obo/UO_0000060>
    
    
Class: <http://purl.obolibrary.org/obo/UO_0010008>

    Annotations: 
        rdfs:isDefinedBy <http://purl.obolibrary.org/obo/uo.owl>,
        rdfs:label "kilometer per hour"
    
    SubClassOf: 
        <http://purl.obolibrary.org/obo/UO_0000060>
    
    
Class: <http://purl.obolibrary.org/obo/uo.owl/unit>

    Annotations: 
        rdfs:comment "reused from Units of measurement Ontology"^^xsd:string,
        rdfs:isDefinedBy <http://purl.obolibrary.org/obo/uo.owl>
    
    SubClassOf: 
        toco:ConceptEntities
    
    
Class: <http://purl.org/vocommons/voaf#Vocabulary>

    
Class: <http://www.w3.org/2003/01/geo/wgs84_pos#Point>

    Annotations: 
        rdfs:comment "The relation between something and the point, 
 or other geometrical thing in space, where it is.  For example, the realtionship between
 a radio tower and a Point with a given lat and long.
 Or a relationship between a park and its outline as a closed arc of points, or a road and
 its location as a arc (a sequence of points).
 Clearly in practice there will be limit to the accuracy of any such statement, but one would expect
 an accuracy appropriate for the size of the object and uses such as mapping .",
        rdfs:isDefinedBy <http://www.w3.org/2003/01/geo/wgs84_pos#>,
        rdfs:label "location"
    
    SubClassOf: 
        <http://www.w3.org/2003/01/geo/wgs84_pos#SpartialThing>
    
    
Class: <http://www.w3.org/2003/01/geo/wgs84_pos#SpartialThing>

    Annotations: 
        rdfs:isDefinedBy <http://www.w3.org/2003/01/geo/wgs84_pos#>
    
    SubClassOf: 
        toco:ConceptEntities
    
    
Class: foaf:Person

    Annotations: 
        rdfs:isDefinedBy <http://xmlns.com/foaf/0.1/>
    
    SubClassOf: 
        toco:ConceptEntities
    
    
Class: om:ObervationAndMeasurement

    Annotations: 
        rdfs:comment "reused from SenSei Observation And Measurement Ontology (http://purl.oclc.org/net/unis/ontology/sensordata.owl)."^^xsd:string,
        rdfs:isDefinedBy <http://purl.oclc.org/net/unis/ontology/sensordata.owl>
    
    SubClassOf: 
        toco:ConceptEntities
    
    
Class: toco:AccessPoint

    Annotations: 
        rdfs:comment "a wireless access point, or more generally just access point (AP), is a networking hardware device that allows a Wi-Fi/Li-Fi device to connect to a wired network. The AP usually connects to a router (via a wired network) as a standalone device, but it can also be an integral component of the router itself. An AP is differentiated from a hotspot, which is the physical location where Wi-Fi access to a WLAN is available."^^xsd:string
    
    SubClassOf: 
        toco:SystemDevice
    
    
Class: toco:Action

    Annotations: 
        rdfs:comment "the action of a flow defined in OpenFlow protocol"
    
    SubClassOf: 
        toco:ConceptEntities
    
    
Class: toco:Attached

    SubClassOf: 
        toco:UserDeviceStatus
    
    
Class: toco:AudioService

    SubClassOf: 
        toco:Service
    
    
Class: toco:AudioSession

    SubClassOf: 
        toco:Session
    
    
Class: toco:BaseStation

    Annotations: 
        rdfs:comment "a \"land station in the land mobile service.\" -- according to the International Telecommunication Union's (ITU) Radio Regulations (RR).

it is a transceiver connecting a number of other devices to one another and/or to a wider area. In LTE, it is also known as eNodeB."^^xsd:string
    
    SubClassOf: 
        toco:SystemDevice
    
    
Class: toco:CellularUserEquipment

    Annotations: 
        rdfs:comment "User deivce in a Cellular network."^^xsd:string
    
    SubClassOf: 
        toco:UserEquipment
    
    
Class: toco:ConceptEntities

    DisjointWith: 
        toco:PhysicalInfrastructure
    
    
Class: toco:Detached

    SubClassOf: 
        toco:UserDeviceStatus
    
    
Class: toco:Device

    Annotations: 
        rdfs:comment "represent all the devices in the physical infrastructure of telecommunciation system. 

According to its user, could be divided into UserDevice and SystemDevice."^^xsd:string
    
    SubClassOf: 
        toco:PhysicalInfrastructure
    
    
Class: toco:Drop

    SubClassOf: 
        toco:Action
    
    
Class: toco:FileTransferService

    SubClassOf: 
        toco:Service
    
    
Class: toco:Flow

    Annotations: 
        rdfs:comment "the flow entry in a flow table inside a switch or route. Defined by OpenFlow protocol."
    
    SubClassOf: 
        toco:ConceptEntities
    
    
Class: toco:Forward

    SubClassOf: 
        toco:Action
    
    
Class: toco:Host

    Annotations: 
        rdfs:comment "A host is a computer or other device connected to a computer network. It is a network node that is assigned a network address."^^xsd:string
    
    SubClassOf: 
        toco:UserDevice
    
    
Class: toco:Interface

    SubClassOf: 
        toco:PhysicalInfrastructure
    
    
Class: toco:LTEAssociation

    Annotations: 
        rdfs:comment "the electromagnetic wave carring modulated signal between LTE base station, or eNodeB, and user equipment"^^xsd:string
    
    SubClassOf: 
        toco:WirelessAssociation
    
    
Class: toco:LiFiAccessPoint

    Annotations: 
        rdfs:comment "The access point in Li-Fi network. Li-Fi is a wireless optical networking technology that uses light-emitting diodes (LEDs) for data transmission."^^xsd:string
    
    SubClassOf: 
        toco:AccessPoint
    
    
Class: toco:LiFiAssociation

    Annotations: 
        rdfs:comment "the visiable light carring modulated signals in Li-Fi network. Transmited and received by LiFi user equipment and LiFi access point."^^xsd:string
    
    SubClassOf: 
        toco:WirelessAssociation
    
    
Class: toco:LiFiUserEquipment

    Annotations: 
        rdfs:comment "any device used directly by an end-user to communicate. It can be a hand-held telephone, a laptop computer equipped with a mobile broadband adapter, or any other device."^^xsd:string
    
    SubClassOf: 
        toco:UserEquipment
    
    
Class: toco:LiFiWLAN

    Annotations: 
        rdfs:comment "WLAN interface on the devices in LIFi network, e.g., LiFi user equipment, LiFi access point."^^xsd:string
    
    SubClassOf: 
        toco:WLAN
    
    
Class: toco:Link

    SubClassOf: 
        toco:PhysicalInfrastructure
    
    
Class: toco:Output

    SubClassOf: 
        toco:Action
    
    
Class: toco:PathFlow

    SubClassOf: 
        toco:Flow
    
    
Class: toco:PhysicalInfrastructure

    Annotations: 
        rdfs:comment "Describe all the physical resources in a telecommunication network system, which is divided into three main modules, namely, device, interface, link. 

Please be reminded the electromagnetic wave (which is the links of all wireless communication netwoks), even if it is invisable, physically exists. Thus, it is also described in the subclass of \"net;PhysicalInfrastructure\"."^^xsd:string
    
    DisjointWith: 
        toco:ConceptEntities
    
    
Class: toco:SatelliteAssociation

    Annotations: 
        rdfs:comment "the milli-meter electromagnetic wave carring modulated signal between satellite base stations and ground station."^^xsd:string
    
    SubClassOf: 
        toco:WirelessAssociation
    
    
Class: toco:SatelliteGroundStation

    Annotations: 
        rdfs:comment "used in satellite network. Also known as earth station, or earth terminal, it is a terrestrial radio station designed for extraplanetary telecommunication with spacecraft (constituting part of the ground segment of the spacecraft system), or reception of radio waves from astronomical radio sources. Ground stations may be located either on the surface of the Earth, or in its atmosphere.[1] Earth stations communicate with spacecraft by transmitting and receiving radio waves in the super high frequency or extremely high frequency bands (e.g., microwaves). When a ground station successfully transmits radio waves to a spacecraft (or vice versa), it establishes a telecommunications link. A principal telecommunications device of the ground station is the parabolic antenna."^^xsd:string
    
    SubClassOf: 
        toco:UserEquipment
    
    
Class: toco:SatelliteRelayStation

    Annotations: 
        rdfs:comment "An artificial satellite, that relays and amplifies radio telecommunications signals via a transponder; it creates a communication channel between a source transmitter and a receiver at different locations on Earth. Communications satellites are used for television, telephone, radio, internet, and military applications."^^xsd:string
    
    SubClassOf: 
        toco:SystemDevice
    
    
Class: toco:Service

    Annotations: 
        rdfs:comment "a communication service, e.g., voice, video, file uploading/downloading, etc."^^xsd:string
    
    SubClassOf: 
        toco:ConceptEntities
    
    
Class: toco:Session

    SubClassOf: 
        toco:ConceptEntities
    
    
Class: toco:Switch

    Annotations: 
        rdfs:comment "A network switch (also called switching hub, bridging hub, officially MAC bridge) is a computer networking device that connects devices together on a computer network by using packet switching to receive, process, and forward data to the destination device."^^xsd:string
    
    SubClassOf: 
        toco:SystemDevice
    
    
Class: toco:SystemDevice

    Annotations: 
        rdfs:comment "All the physical facilities in the telecommunication system that provide the communication service to uses. For example: base station towers, Wi-Fi access points, switches, servers, etc."^^xsd:string
    
    SubClassOf: 
        toco:Device
    
    
Class: toco:Text

    SubClassOf: 
        toco:Service
    
    
Class: toco:User

    Annotations: 
        rdfs:comment "reused from foaf (http://xmlns.com/foaf/0.1/). Represent a user in the telecommunication system."^^xsd:string
    
    SubClassOf: 
        foaf:Person
    
    
Class: toco:UserDevice

    Annotations: 
        rdfs:comment "User Devices, requiring connectivity services, e.g., phones, tablets, laptops, wearable devices, etc."^^xsd:string
    
    SubClassOf: 
        toco:Device
    
    
Class: toco:UserDeviceStatus

    SubClassOf: 
        toco:ConceptEntities
    
    
Class: toco:UserEquipment

    Annotations: 
        rdfs:comment "any device used directly by an end-user to communicate. It can be a hand-held telephone, a laptop computer equipped with a mobile broadband adapter, or any other device."^^xsd:string
    
    SubClassOf: 
        toco:UserDevice
    
    
Class: toco:VideoService

    SubClassOf: 
        toco:Service
    
    
Class: toco:VideoSession

    SubClassOf: 
        toco:Session
    
    
Class: toco:WLAN

    Annotations: 
        rdfs:comment "A wireless local area network (WLAN) interface, also known as WLAN, is the interface of a wireless computer network that links two or more devices using wireless communication within a limited area such as a home, school, computer laboratory, or office building."
    
    SubClassOf: 
        toco:Interface
    
    
Class: toco:WiFiAccessPoint

    Annotations: 
        rdfs:comment "An access point in a WiFi network"^^xsd:string
    
    SubClassOf: 
        toco:AccessPoint
    
    
Class: toco:WiFiAssociation

    Annotations: 
        rdfs:comment "the electromagnetic wave carring modulated signal between LTE base station, or eNodeB, and user equipment"^^xsd:string
    
    SubClassOf: 
        toco:WirelessAssociation
    
    
Class: toco:WiFiUserEquipment

    Annotations: 
        rdfs:comment "a user quipment in Wi-Fi network"^^xsd:string
    
    SubClassOf: 
        toco:UserEquipment
    
    
Class: toco:WiFiWLAN

    Annotations: 
        rdfs:comment "WLAN interface on the devices in LIFi network, e.g., LiFi user equipment, LiFi access point."^^xsd:string
    
    SubClassOf: 
        toco:WLAN
    
    
Class: toco:WiredLink

    Annotations: 
        rdfs:comment "wired link through twisted cable, optical fiber, etc."
    
    SubClassOf: 
        toco:Link
    
    DisjointWith: 
        toco:WirelessAssociation
    
    
Class: toco:WirelessAssociation

    Annotations: 
        rdfs:comment "the electromeganetic radio transmiting through wireless channels in wireless network, carring communication data. Depend on its frequency, it could be visiable light, micro waves, radio waves."^^xsd:string
    
    SubClassOf: 
        toco:Link
    
    DisjointWith: 
        toco:WiredLink
    
    
Class: toco:unReachable

    SubClassOf: 
        toco:UserDeviceStatus
    
    
Individual: toco:

    Types: 
        <http://purl.org/vocommons/voaf#Vocabulary>
    
    
